\documentclass[11pt]{scrartcl}

\usepackage{cancel}
\usepackage[utf8]{inputenc}
\usepackage{mathtools}
\usepackage[sexy]{evan}

\title{04RUS113}
\author{Himadri Mandal}

\begin{document}
\maketitle

\section{Solution}
\begin{soln}
Let $\deg Q = m, \deg P = n$, and let $\zeta_k$ be a $k$th root of unity.
\begin{claim*}
$m \mid n$
\end{claim*}
\begin{proof}
  Let $R \in \RR[x,y]$ such that
  \[ (Q(x) - Q(y))\cdot R(x,y) = P(x) - P(y) \]
  Clearly, $\deg(R) = n - m$. Setting $x = \zeta_m x, y = x$,
  \[ (Q(\zeta_m x) - Q(x))R(\zeta_m x,x) = P(\zeta_mx) - P(x)\]
  As $\deg (Q(\zeta_m x) - Q(x)) \leq m-1 \implies \deg(P(\zeta_mx) - P(x)) \leq n-1$.
  Therefore, $x^n(\zeta_m^n - 1) = 0 \ \forall \ x \in \CC$. So $m \mid n$.
   
\end{proof}
\hrule

\bigskip
To finish, WLOG assume leading coeffs of $P,Q$ are $1$, now we will induct on the degree, base case is clear. 
  \[ Q(x) - Q(y) \mid (P(x) - Q(x)) - (P(y) - Q(y)),\] 
  which has degree $n - m$. By hypothesis, $P(x) - Q(x) = S_1(Q(x))$. 
  Now, taking $S(x) = S_1(x) + x$, we would have $P(x) = S(Q(x))$.
\end{soln}
\end{document}

