\documentclass[11pt]{scrartcl}

\usepackage{cancel}
\usepackage[utf8]{inputenc}
\usepackage{mathtools}
\usepackage[sexy]{evan}

\title{21CMIMCA5}
\author{Himadri Mandal}

\begin{document}
\maketitle

\section{Solution}
\begin{soln}
Define $g(x) = f(x) + f(43 + x) + \cdots + f(46 \cdot 43 + x)$, $g(x+43) - g(x) 
= f(2017 + x) - f(x)$, so we wanna find $g(43) - g(0)$. $g(x) = (-2)^x$ for $0 \leq x \leq 42$,
which would be equivalent to 
\[ (1-3)^x = \binom{x}{0} - \binom{x}{1}3^1 + \cdots + \binom{x}{42}3^{42} = g(x)\]
now $g(43) = (-2)^{43} + \binom{43}{43}3^{43}$, thus the final answer is $3^{43}-2^{43}-1$.
\end{soln}
\end{document}
