\documentclass[11pt]{scrartcl}

\usepackage{cancel}
\usepackage[utf8]{inputenc}
\usepackage{mathtools}
\usepackage[sexy]{evan}

\title{14TSTST6}
\author{Himadri Mandal}

\begin{document}
\maketitle

\section{Solution}

\raggedright
\begin{soln}
  Could not solve it but found it instructive. Let $\alpha$ be the first integer such that $p|ca^\alpha - db^\alpha$, $\lambda$ is the order of $a/b$.
\[ \nu_p \left( c a^{\alpha + n\lambda} - d b^{\alpha + n \lambda} \right)
	= \nu_p \left(
		\left( \frac{a^\lambda}{b^\lambda} \right)^n
		- \frac{d a^\alpha}{c b^{\alpha}} \right)
\]
to be constant.
\begin{proposition*}
	$x \equiv y \equiv 1 \pmod p$.
	If the sequence $\nu_p\left( x^n - y \right)$ of positive integers
	is nonconstant, then it is unbounded.
\end{proposition*}

\begin{claim*}
	Suppose $m$ and $n$ are positive integers such that
	\[ d = \nu_p(x^n-y) < \nu_p(x^m-y) = e. \]
	Then there exists $\ell$ such that $\nu_p(x^\ell - y) \ge e + 1$.
\end{claim*}
\begin{proof}
$\nu_p(x^m - x^n) = \nu_p\left( (x^m-y) - (x^n-y) \right) = d$
\[ \nu_p(x^k-1) = e \]
for $k = p^{e-d}|m-n|$.
Now we set $x^k = p^e u + 1$ and $x^m = p^e v + y$. Thus we get for $1 \le r \le p-1$
\begin{align*}
	x^{kr+m}-y &= (p^e u + 1)^r \cdot (p^e v + y) - y \\
	&= p^e \left( v + yu \cdot r \right) + p^{2e} \left( \dots \right).
\end{align*}
  Choosing $r$ with $r \equiv -\frac{v}{u} \pmod p$,
we have $p^{e+1} \mid x^{kr+m} - y$,
hence $\ell = kr+m$ proves the claim.
\end{proof}

This proves the proposition but as it was equivalent to the problem, we are done.
\end{soln}

\end{document}
