\documentclass[11pt]{scrartcl}

\usepackage{cancel}
\usepackage[utf8]{inputenc}
\usepackage{mathtools}
\usepackage[sexy]{evan}

\title{14PTNMB4}
\author{Himadri Mandal}

\begin{document}
\maketitle

\section{Solution}
\newcommand{\sgn}{\operatorname{sgn}}
\begin{soln}
  Note that 
  \[ P(x) = \sum_{k = 0}^{n} \frac{(2^n \cdot x)^k}{2^{k^2}} \]
  Obviously, $P(x)$ can be replaced with $P(\frac{x}{2^n})$.
\begin{claim*}
  Consider the sequence $a_i = 2i, 0 \leq i \leq n$. Then, $\sgn(P(-2^{a_i})) = (-1)^i$. 
\end{claim*}
\begin{proof}
  Notice that $|\pm 2^m| > |\sum_{k = 0}^{m-1} \pm 2^k|$, thus 
  \[ \sgn(P(-2^{a_i})) = \sgn \left(\sum_{k=0}^{n} (-1)^k \cdot2^{k(a_i - k)} \right) = \sgn((-1)^k)\]
  such that $k(a_i-k)$ is the biggest, this might not work when there are atleast two of the same terms
  but this cannot happen because $a_i$ is even.
  To finish note that $k(a_i - k) = k(2i - k)$ achieves maximum at $k = i$, so 
  $\sgn(P(-2^{a_i})) = (-1)^i$
\end{proof}
\hrule
\bigskip
  Now by IVT $P$ has atleast $n$ real roots, so all roots of $P$ are real.
\end{soln}
\end{document}

