\documentclass[11pt]{scrartcl}

\usepackage{cancel}
\usepackage[utf8]{inputenc}
\usepackage{mathtools}
\usepackage[sexy]{evan}

\title{68PTNMA6}
\author{Himadri Mandal}

\begin{document}
\maketitle

\section{Solution}
\begin{soln}
Let the roots be $\lambda_1,\cdots, \lambda_n$, then $\sum_i \lambda_i^2 = a_{n-1}^2 - 2a_{n-2} = 3$
  but also by AMGM $\prod_i \lambda_i^2 = 1 \implies \sum_i \lambda_i^2 \geq n \sqrt{\prod_i \lambda_i^2}$.
  So, $n = \{3,2,1\}$. For $n = 3$, checking $\{x^3 \pm x^2 -x \pm 1\}$ we see that $P(x) = x^3 -x \pm(x^2 - 1)$ work.
  $n = 2,1$ are easy. So the final set of solutions are $P(x) = \{x \pm 1, x^2 -1 \pm x, x^3 - x \pm(x^2 -1)\}$
\end{soln}
\end{document}
